

Assignment 4

(1) For stability, TF of system must contain $j\omega$ axis in its ROC.

(2) $x(t) = \underbrace{e^{-3t} u(t-2)}_{\text{1st term}} - \underbrace{e^{5t} u(4-t)}_{\text{2nd term}}$

$$\begin{aligned} & \text{1st term} \\ & e^{-3(t-2)} u(t-2) e^{-6} \\ & = e^{-6} e^{-3(t-2)} u(t-2). \end{aligned}$$

$$\begin{aligned} e^{-at} u(t) & \rightarrow \frac{1}{s+a} & e^{-at} u(t) & \rightarrow \frac{1}{s+a} \\ x(t) & \rightarrow X(s) \\ x(t-t_0) & \rightarrow e^{-s t_0} X(s). \end{aligned}$$

$$\begin{aligned} & \rightarrow \frac{e^{-3(t-2)} u(t-2)}{e^{-6}} \rightarrow \frac{1}{(s+3)} e^{-2s} \times e^{-6} \end{aligned}$$

$$= \frac{e^{-2s} e^{-6}}{(s+3)} \quad \text{Re}\{s\} > -3.$$

$$-e^{5t} u(4-t)$$

$$= -e^{20} e^{5t} e^{-20} u(4-t)$$

$$= -e^{20} e^{5(t-4)} u(4-t)$$

$$= -e^{20} e^{5(t-4)} u(-(t-4))$$

$$= -e^{20} e^{-\alpha t} u(-t)$$

$$\begin{aligned} -\alpha &= 5 & \hookrightarrow & = e^{20} \frac{1}{s+\alpha} \quad \text{Re}\{s\} < -\alpha. \\ \alpha &= -5 & & \end{aligned}$$

$$= e^{20} \frac{1}{s-\alpha} \quad \text{Re}\{s\} < 5$$

$$= e^{20} \frac{1}{s-5} e^{-4s} \quad \text{Re}\{s\} < 5$$

$$\therefore \text{LT} = \frac{e^{-6} e^{-2s}}{s+3} + \frac{e^{20} e^{-4s}}{s-5} \quad \text{ROC} \\ -3 < \text{Re}\{s\} < 5$$

$$(3) \quad e^{-at} u(-t) \rightarrow \frac{1}{s+a}, \quad \text{Re}\{s\} < -a$$

$$+ t x(t) \rightarrow -\frac{d x(s)}{ds}$$

$$\underbrace{e^{-at} u(-t)}_{x(t)} \rightarrow \underbrace{\frac{-1}{s+a}}_{x(s)} \quad \text{Re}\{s\} < -a$$

$$t x(t) \rightarrow -\left[\frac{d}{ds} x(s) \right]$$

$$\underbrace{x(t)}_{x_1(t)} \rightarrow \underbrace{x(s)}_{x_1(s)}$$

$$t x_1(t) \rightarrow -\frac{d}{ds} x_1(s)$$

$$\Rightarrow t t x(t) \rightarrow -\frac{d}{ds} \left[-\frac{d}{ds} x(s) \right]$$

$$t^2 x(t) = \frac{d^2}{ds^2} x(s)$$

$$= \frac{d^2}{ds^2} \left(\frac{-1}{s+a} \right)$$

$$= \frac{d}{ds} \left[-1 \left(\frac{(s+a) \cdot 0 - 1 \cdot 1}{(s+a)^2} \right) \right]$$

$$= \frac{d}{ds} \left[\frac{1}{(s+a)^2} \right]$$

$$= \frac{(s+a)^2 \cdot 0 - 2(s+a)}{(s+a)^4}$$

$$= \frac{-2}{(s+a)^3} \quad \checkmark$$

$$(4) \quad \sin(at) \rightarrow \frac{a}{s^2 + a^2}$$

$$\sin(-at) \rightarrow \frac{-a}{s^2 + a^2}$$

$$(5) \quad x(t) \rightarrow X(s)$$

$$x(-t) \rightarrow X(-s)$$

$$t x(-t) \rightarrow \frac{-1}{ds} x(-s)$$

$$(6) e^{-at} u(t) \rightarrow \frac{1}{s+a}, \operatorname{Re}\{s\} > -a$$

$$-e^{-at} u(-t) \rightarrow \frac{1}{s+a}, \operatorname{Re}\{s\} < -a$$

$$(7) e^{-at} u(-t) \rightarrow \frac{-1}{s+a}, \operatorname{Re}\{s\} < -a$$

$$e^{-2t} u(t) \rightarrow \frac{1}{s+2}, \operatorname{Re}\{s\} > -2$$

$$e^{4t} u(t) \rightarrow \frac{-1}{s-4}, \operatorname{Re}\{s\} < 4$$

$$\frac{1}{s+2} - \frac{1}{s-4}$$

$$= \frac{s-4 - s-2}{(s+2)(s-4)}$$

$$= \frac{-6}{(s+2)(s-4)} \quad -2 < \operatorname{Re}\{s\} < 4$$

$$(7) \frac{y(s)}{x(s)} = s^2 + 2s + 1$$

$$y(s) = (s^2 x(s) + 2s x(s) + x(s))$$

$$y(t) = \frac{d^2 x(t)}{dt^2} + 2 \frac{dx(t)}{dt} + x(t)$$

A LCCDE involving $x(t)$, $y(t)$ & and higher order derivatives of $x(t)$ only.

$$(8) x(t) \rightarrow x(s)$$

$$x(at) \rightarrow \frac{1}{|a|} x(s/a)$$

$$x(t/s) \rightarrow s x(s)$$

$$a = 1/5$$

$$x(-t/5) \rightarrow \underline{s x(-5s)}$$

$$(9) e^{-3t} u(t-4)$$

$$= e^{-3t} e^{+3 \cdot 4} e^{-3 \cdot 4} u(t-4)$$

$$= e^{-3(t-4)} e^{-12} u(t-4)$$

$$= e^{-12} e^{-3(t-4)} u(t-4)$$

$$\frac{e^{-at} u(t)}{u(t)} \rightarrow \frac{1}{s+a}$$

$$u(t-4) \rightarrow \frac{e^{-4s}}{s+3} e^{-12}$$

$$\operatorname{Re}\{s\} > \underline{-3}$$

$$-e^{-at} u(-t) \rightarrow \frac{1}{s+a} \quad \operatorname{Re}\{s\} < -a$$

$$-e^{-2t} u(2-t) = -e^{-2t} e^{2 \cdot 2} u(2-t)$$

$$= -e^{-2(t-2)} e^{-4} u(2-t) \quad e^4$$

$$= -e^{-2(t-2)} u(-(t-2)) e^{-4}$$

$$-e^{-at} u(-t) \rightarrow \frac{1}{s+a} \quad \operatorname{Re}\{s\} < -a$$

$$a = -2$$

$$-e^{+2t} u(-t) \rightarrow \frac{1}{s-a} \quad \operatorname{Re}\{s\} < 2$$

$$= -e^{2(t-2)} u(-(t-2)) \rightarrow \frac{e^{-4s}}{s-2} e^{-4}$$

L.T

$$= \frac{e^{-12} e^{-4s}}{s+3} + \frac{e^4 e^{-2s}}{s-2}$$

$$-3 < \operatorname{Re}\{s\} < 2$$

$$(10) \frac{1}{s-a} \rightarrow \operatorname{Re}\{s\} > a$$

$$e^{at} u(t) \rightarrow \frac{1}{s-a}, \operatorname{Re}\{s\} > \underline{a}$$